theories/lifting.v
@@ -385,11 +385,12 @@ Section lifting.
 
   Lemma wp_read_mem n len a vread (vmem : bv n) es ann kind tag q:
     n = (8 * len)%N →
+    0 < Z.of_N len →
     a ↦ₘ{q} vmem -∗
     (⌜vread = vmem⌝ -∗ a ↦ₘ{q} vmem -∗ WPasm es) -∗
     WPasm (ReadMem (Val_Bits (BVN n vread)) kind (Val_Bits (BVN 64 a)) len tag ann :: es).
   Proof.
-    iIntros (?) "Hm Hcont". setoid_rewrite wp_asm_unfold. subst.
+    iIntros (??) "Hm Hcont". setoid_rewrite wp_asm_unfold. subst.
     iIntros ([???]) "/= -> -> Hθ".
     iApply wp_lift_step; [done|].
     iIntros (σ1 ????) "(Hctx&Hictx&Hmem)".
@@ -402,7 +403,7 @@ Section lifting.
     }
     iIntros "!>" (????). iMod "HE" as "_". iModIntro.
     inv_seq_step.
-    revert select (∃ _, _) => -[?[?[?[?[?[?[?[?[[??]|?]]]]]]]]]; simplify_eq/=. 2:{
+    revert select (∃ _, _) => -[?[?[?[?[?[?[?[?[?[[??]|?]]]]]]]]]]; simplify_eq/=. 2:{
       iFrame. iSplitL; [|done]. by iApply wp_value.
     }
     iFrame. iSplit; [|done].
@@ -411,11 +412,12 @@ Section lifting.
 
   Lemma wp_write_mem n len a (vold vnew : bv n) es ann res kind tag:
     n = (8 * len)%N →
+    0 < Z.of_N len →
     a ↦ₘ vold -∗
-    (⌜res = true⌝ -∗ a ↦ₘ vnew -∗ WPasm es) -∗
+    (a ↦ₘ vnew -∗ WPasm es) -∗
     WPasm (WriteMem (Val_Bool res) kind (Val_Bits (BVN 64 a)) (Val_Bits (BVN n vnew)) len tag ann :: es).
   Proof.
-    iIntros (?) "Hm Hcont". subst. setoid_rewrite wp_asm_unfold.
+    iIntros (??) "Hm Hcont". subst. setoid_rewrite wp_asm_unfold.
     iIntros ([???]) "/= -> -> Hθ".
     iApply wp_lift_step; [done|].
     iIntros (σ1 ????) "(Hctx&Hictx&Hmem)".
@@ -424,18 +426,43 @@ Section lifting.
     have ? : len' = len by lia. subst.
     iSplit. {
       iPureIntro. eexists _, _, _, _. simpl. econstructor; [done | by econstructor |]. simpl.
-      naive_solver.
+      eexists _, _, _. simplify_option_eq. naive_solver.
     }
     iIntros "!>" (????). iMod "HE" as "_".
     inv_seq_step.
-    revert select ((∃ _, _) ∨ _) => -[[?[?[?[?[?[?[?[??]]]]]]]]|[??]]; simplify_eq/=.
-    2:{
-      iFrame. iSplitL; [|done]. by iApply wp_value.
-    }
+    revert select (∃ _, _) => -[?[?[?[?[??]]]]]; simplify_option_eq; destruct_and!; simplify_eq.
     iMod (mem_mapsto_update with "Hmem Hm") as (len' ?) "[Hmem Hm]".
     have ? : len' = len by lia. subst. iFrame.
     iModIntro. iSplitL; [|done].
-    by iApply ("Hcont" with "[% //] Hm").
+    by iApply ("Hcont" with "Hm").
+  Qed.
+
+  Lemma wp_write_mmio n len a (vnew : bv n) es ann res kind tag κs:
+    n = (8 * len)%N →
+    0 < Z.of_N len →
+    mmio_range a (Z.of_N len) -∗
+    spec_trace (SWriteMem a vnew::κs) -∗
+    (spec_trace κs -∗ WPasm es) -∗
+    WPasm (WriteMem (Val_Bool res) kind (Val_Bits (BVN 64 a)) (Val_Bits (BVN n vnew)) len tag ann :: es).
+  Proof.
+    iIntros (??) "Hm Hspec Hcont". subst. setoid_rewrite wp_asm_unfold.
+    iIntros ([???]) "/= -> -> Hθ".
+    iApply wp_lift_step; [done|].
+    iIntros (σ1 ????) "(Hctx&Hictx&Hmem)".
+    iApply fupd_mask_intro; first set_solver. iIntros "HE".
+    iDestruct (mmio_range_lookup with "Hmem Hm") as %Hread; [done|].
+    rewrite N2Z.id in Hread.
+    iDestruct (mmio_range_Forall with "Hmem Hm") as %?.
+    iSplit. {
+      iPureIntro. eexists _, _, _, _. simpl. econstructor; [done | by econstructor |]. simpl.
+      eexists ∅, _, _. simplify_option_eq. naive_solver.
+    }
+    iIntros "!>" (????). iMod "HE" as "_".
+    inv_seq_step.
+    revert select (∃ _, _) => -[?[?[?[?[??]]]]]; simplify_option_eq; destruct_and!; simplify_eq.
+    iMod (spec_ctx_cons with "Hctx Hspec") as "[Hctx Hspec]".
+    iFrame. iModIntro. iSplitL; [|done].
+    by iApply ("Hcont" with "Hspec").
   Qed.
 
   Lemma wp_branch_address v es ann:
